theories/rust_typing/debug.v
@@ -1,0 +1,8 @@
+From refinedrust Require Export automation.
+Set Default Proof Using "Type".
+
+Ltac hooks.shelve_sidecond_hook ::=
+    match goal with
+    | |- False => fail 4
+    | |- _ => idtac
+    end.
