theories/rust_typing/uninit.v
@@ -1,148 +1,9 @@
 From refinedrust Require Export type uninit_def.
-From refinedrust Require Import programs ltype_rules.
+From refinedrust Require Import programs ltype_rules value.
 Set Default Proof Using "Type".
 
-Section typing.
+Section lemmas.
   Context `{!typeGS Σ}.
-
-  (** ** Instances for deinitializing a type *)
-
-  (* Two low-priority instances that trigger as a fallback for ltypes foldable to a ty (no borrows below) *)
-  Lemma owned_subltype_step_ofty_uninit π E L {rt} (lt : ltype rt) r st T :
-    cast_ltype_to_type E L lt (λ ty,
-    li_tactic (compute_layout_goal (ty_syn_type ty)) (λ ly1,
-      li_tactic (compute_layout_goal st) (λ ly2,
-        ⌜ly1 = ly2⌝ ∗ T L (ty_ghost_drop ty π r))))
-    ⊢ owned_subltype_step π E L #r #() lt (◁ uninit st) T.
-  Proof.
-    iDestruct 1 as "(%ty & %Heqt & HT)".
-    rewrite /compute_layout_goal.
-    iDestruct "HT" as "(%ly1 & %Hst1 & %ly2 & %Hst2 & <- & HT)".
-    iIntros (???) "CTX HE HL Hl". simp_ltypes; simpl.
-    iPoseProof (full_eqltype_acc with "CTX HE HL") as "#Hincl"; first apply Heqt.
-    iSpecialize ("Hincl" $! (Owned false) (#r)).
-    iDestruct "Hincl" as "(Hincl & _)". iDestruct "Hincl" as "(%Hst & Hincl & _)".
-    iMod (ltype_incl'_use with "Hincl Hl") as "Hl"; first done.
-    iExists _, _. iFrame.
-    rewrite ltype_own_ofty_unfold /lty_of_ty_own.
-    iDestruct "Hl" as "(%ly & %Halg & %Hly & Hsc & Hlb & _ & %r' & <- & Hb)".
-    assert (ly1 = ly) as -> by by eapply (syn_type_has_layout_inj (ty_syn_type ty)).
-    iMod (fupd_mask_mono with "Hb") as "(%v & Hl & Hv)"; first done.
-    iModIntro. iSplitL.
-    { iPoseProof (ty_own_val_has_layout with "Hv") as "%Hlyv"; first done.
-      iPoseProof (ty_own_ghost_drop with "Hv") as "Hb"; first done.
-      iApply (logical_step_wand with "Hb"). iIntros "$".
-      rewrite ltype_own_ofty_unfold /lty_of_ty_own.
-      iExists _. iR. iR. simpl. iR. iFrame. iR.
-      iExists _. iR. iModIntro. iExists _. iFrame.
-      rewrite uninit_own_spec. eauto. }
-    iPureIntro.
-    iIntros (ly1' ly2' Hst1' Hst2').
-    rewrite Hst in Hst1'. simp_ltypes in Hst1'.
-    assert (ly1' = ly) as -> by by eapply syn_type_has_layout_inj.
-    assert (ly2' = ly) as -> by by eapply syn_type_has_layout_inj.
-    done.
-  Qed.
-  Global Instance owned_subltype_step_ofty_uninit_inst π E L {rt} (lt : ltype rt) r st :
-    OwnedSubltypeStep π E L #r #() lt (◁ uninit st)%I | 101:=
-    λ T, i2p (owned_subltype_step_ofty_uninit π E L lt r st T).
-
-  (* Higher-priority instacne for the special case that we go to Untyped *)
-  Lemma owned_subltype_step_ofty_uninit_untyped π E L {rt} (lt : ltype rt) r ly T :
-    cast_ltype_to_type E L lt (λ ty,
-    ⌜syn_type_has_layout (ty_syn_type ty) ly⌝ ∗ T L (ty_ghost_drop ty π r))
-    ⊢ owned_subltype_step π E L #r #() lt (◁ uninit (UntypedSynType ly)) T.
-  Proof.
-    iDestruct 1 as "(%ty & %Heqt & HT)".
-    iDestruct "HT" as "(%Hst & HT)".
-    iApply owned_subltype_step_ofty_uninit.
-    iExists ty. iR.
-    iExists ly. iR. iExists ly.
-    iSplitR. { iPureIntro. by eapply syn_type_has_layout_make_untyped. }
-    iR. done.
-  Qed.
-  Global Instance owned_subltype_step_ofty_uninit_untyped_inst π E L {rt} (lt : ltype rt) r ly :
-    OwnedSubltypeStep π E L #r #() lt (◁ uninit (UntypedSynType ly))%I | 100 :=
-    λ T, i2p (owned_subltype_step_ofty_uninit_untyped π E L lt r ly T).
-
-  (* More specific instances *)
-  Lemma owned_subltype_step_shrltype_uninit π E L {rt} (lt : ltype rt) r st κ T  :
-    ⌜syn_type_compat PtrSynType st⌝ ∗ T L True%I
-    ⊢ owned_subltype_step π E L r #() (ShrLtype lt κ) (◁ uninit st) T.
-  Proof.
-    iIntros "(%Hstcomp & HT)".
-    iIntros (???) "CTX HE HL Hl". simp_ltypes; simpl.
-    iMod (ltype_deinit_shr with "Hl") as "Hl"; [done.. | ].
-    iExists _, _. iFrame.
-    iSplitL. { iApply logical_step_intro. by iFrame. }
-    iModIntro. iPureIntro. intros ?? Hst1 Hst2.
-    destruct Hstcomp as [<- | (ly1' & Hst' & ->)]; first by eapply syn_type_has_layout_inj.
-    eapply syn_type_has_layout_untyped_inv in Hst2 as (<- & _).
-    by eapply syn_type_has_layout_inj.
-  Qed.
-  Global Instance owned_subltype_step_shrltype_uninit_inst π E L {rt} (lt : ltype rt) r st κ :
-    OwnedSubltypeStep π E L (r) #() (ShrLtype lt κ) (◁ uninit st)%I | 20 :=
-    λ T, i2p (owned_subltype_step_shrltype_uninit π E L lt r st κ T).
-
-  Lemma owned_subltype_step_mutltype_uninit π E L {rt} (lt : ltype rt) r γ st κ T  :
-    match ltype_uniq_extractable lt with
-    | None => False
-    | Some κm =>
-        ⌜syn_type_compat PtrSynType st⌝ ∗ T L (MaybeInherit κm InheritGhost (place_rfn_interp_mut_extracted r γ))
-    end
-    ⊢ owned_subltype_step π E L #(r, γ) #() (MutLtype lt κ) (◁ uninit st) T.
-  Proof.
-    iIntros "HT".
-    iIntros (???) "CTX HE HL Hl". simp_ltypes; simpl.
-    destruct (ltype_uniq_extractable lt) eqn:Hextract; last done.
-    iDestruct "HT" as "(%Hstcomp & HT)".
-    iExists _, _. iFrame.
-    iMod (ltype_uniq_extractable_deinit_mut with "Hl") as "(Hl & Hf)"; [done.. | ].
-    iPoseProof (MaybeInherit_update (place_rfn_interp_mut_extracted r γ) with "[] Hf") as "Hf".
-    { iIntros (?) "Hrfn". iMod (place_rfn_interp_mut_extract with "Hrfn") as "?". done. }
-    iModIntro. iSplitL. { iApply logical_step_intro. iFrame. }
-    iPureIntro. iIntros (ly1 ly2 Halg1 Halg2).
-    specialize (syn_type_compat_layout_trans _ _ _ Hstcomp Halg2) as ?.
-    by eapply syn_type_has_layout_inj.
-  Qed.
-  Global Instance owned_subltype_step_mutltype_uninit_inst π E L {rt} (lt : ltype rt) r γ st κ :
-    OwnedSubltypeStep π E L #(r, γ) #() (MutLtype lt κ) (◁ uninit st)%I | 20 :=
-    λ T, i2p (owned_subltype_step_mutltype_uninit π E L lt r γ st κ T).
-
-  (*Lemma owned_subltype_step_cast_to_type_uninit : *)
-    (*cast_ltype_to_type E L lt (λ ty, *)
-      (*⌜syn_type_compat (ty_syn_type ty) st⌝ ∗ T L (ty_ghost_drop ty)) -∗*)
-    (*owned_subltype_step π E L r #() lt (◁ uninit st) T.*)
-
-  (* TODO have fallback instance that uses cast_ltype *)
-
-  (* TODO more instances for other ltypes under which borrows can happen, e.g. for structs *)
-
-  (* Fallback without a logical step -- here, we cannot ghost_drop *)
-  (* TODO: maybe restrict this instance more for earlier failure *)
-  Lemma uninit_mono E L l {rt} (ty : type rt) r π st T :
-    (li_tactic (compute_layout_goal st) (λ ly, ⌜syn_type_has_layout ty.(ty_syn_type) ly⌝ ∗ (∀ v, v ◁ᵥ{π} r @ ty -∗ T L True%I)))
-    ⊢ subsume_full E L false (l ◁ₗ[π, Owned false] #r @ (◁ ty)) (l ◁ₗ[π, Owned false] .@ (◁ (uninit st))) T.
-  Proof.
-    rewrite /compute_layout_goal.
-    iIntros "(%ly & %Halg1 & %Halg2 & HT)".
-    iIntros (???) "#CTX #HE HL Hl".
-    rewrite !ltype_own_ofty_unfold /lty_of_ty_own. simpl.
-    iDestruct "Hl" as "(%ly' & %Halg & %Hly & Hsc & ? & ? & %r' & <- & Hv)".
-    iMod (fupd_mask_mono with "Hv") as "(%v & Hl & Hv)"; first done.
-    iPoseProof (ty_own_val_has_layout with "Hv") as "%"; first done.
-    iExists L, True%I. iPoseProof ("HT" with "Hv") as "$". iFrame "HL".
-    rewrite right_id. assert (ly' = ly) as -> by by eapply syn_type_has_layout_inj.
-    rewrite ltype_own_ofty_unfold /lty_of_ty_own. simpl.
-    iExists ly. iSplitR; first done. iSplitR; first done.
-    iSplitR; first done. iFrame. iExists _. iSplitR; first done.
-    iModIntro. iModIntro. iExists v. iFrame.
-    iExists ly. iSplitR; first done. iSplitR; first done.
-    iPureIntro. rewrite Forall_forall. done.
-  Qed.
-  Global Instance uninit_mono_inst π E L l {rt} (ty : type rt) (r : rt) st :
-    SubsumeFull E L false (l ◁ₗ[π, Owned false] PlaceIn r @ (◁ ty))%I (l ◁ₗ[π, Owned false] .@ ◁ (uninit st))%I | 40 :=
-    λ T, i2p (uninit_mono E L l ty r π st T).
 
   (* TODO move *)
   Lemma ofty_owned_subtype_aligned π {rt1 rt2} (ty1 : type rt1) (ty2 : type rt2) r1 r2 ly2 l  :
@@ -184,6 +45,19 @@ Section typing.
     by iApply "Hvi".
   Qed.
 
+  Lemma owned_type_incl_uninit' π {rt1} (r1 : rt1) r2 (ty1 : type rt1) st ly :
+    syn_type_size_eq (ty_syn_type ty1) st →
+    syn_type_has_layout st ly →
+    ⊢ owned_type_incl π r1 r2 ty1 (uninit st).
+  Proof.
+    iIntros (Hst ?). iSplitR; last iSplitR.
+    - iPureIntro. done.
+    - simpl. eauto.
+    - iIntros (v) "Hv". iEval (rewrite /ty_own_val/=).
+      iPoseProof (ty_has_layout with "Hv") as "(%ly' & %Hst' & %Hly)".
+      iExists ly. iR. iSplitR. { iPureIntro. rewrite /has_layout_val Hly. apply Hst; done. }
+      iPureIntro. eapply Forall_forall.  eauto.
+  Qed.
   Lemma owned_type_incl_uninit π {rt1} (r1 : rt1) r2 (ty1 : type rt1) st :
     st = ty_syn_type ty1 →
     ⊢ owned_type_incl π r1 r2 ty1 (uninit st).
@@ -197,6 +71,256 @@ Section typing.
       iExists ly. subst st. iR.  iR. iPureIntro.
       eapply Forall_forall.  eauto.
   Qed.
+
+End lemmas.
+
+Section typing.
+  Context `{!typeGS Σ}.
+
+  (** ** Instances for deinitializing a type *)
+
+  (*
+li_tactic (compute_layout_goal (ty_syn_type ty1)) (λ ly1,
+      (* augment context *) ⌜syn_type_has_layout (ty_syn_type ty1) ly1⌝ -∗
+      li_tactic (compute_layout_goal (ty_syn_type ty2)) (λ ly2,
+        (* augment context *) ⌜syn_type_has_layout (ty_syn_type ty2) ly2⌝ -∗
+        ⌜l `has_layout_loc` ly1⌝ -∗ ⌜l `has_layout_loc` ly2⌝ ∗ owned_subtype π E L false r1 r2 ty1 ty2 (λ L', T L' True%I)))
+        *)
+
+  (* Two low-priority instances that trigger as a fallback for ltypes foldable to a ty (no borrows below) *)
+  Lemma owned_subltype_step_ofty_uninit π E L {rt} (lt : ltype rt) r st l T :
+    cast_ltype_to_type E L lt (λ ty,
+    li_tactic (compute_layout_goal (ty_syn_type ty)) (λ ly1,
+      ⌜syn_type_has_layout (ty_syn_type ty) ly1⌝ -∗
+      li_tactic (compute_layout_goal st) (λ ly2,
+        ⌜syn_type_has_layout st ly2⌝ -∗
+        ⌜l `has_layout_loc` ly1⌝ -∗ ⌜l `has_layout_loc` ly2⌝ ∗ 
+        ⌜ly_size ly1 = ly_size ly2⌝ ∗
+        T L (ty_ghost_drop ty π r))))
+    ⊢ owned_subltype_step π E L l #r #() lt (◁ uninit st) T.
+  Proof.
+    iDestruct 1 as "(%ty & %Heqt & HT)".
+    rewrite /compute_layout_goal.
+    iDestruct "HT" as "(%ly1 & %Hst1 & HT)".
+    iDestruct ("HT" with "[//]") as "(%ly2 & %Hst2 & HT)".
+    iIntros (??) "CTX HE HL Hl". simp_ltypes; simpl.
+
+    iPoseProof (full_eqltype_acc with "CTX HE HL") as "#Hincl"; first apply Heqt.
+    iSpecialize ("Hincl" $! (Owned false) (#r)).
+    iDestruct "Hincl" as "(Hincl & _)". iDestruct "Hincl" as "(%Hst & Hincl & _)".
+    iMod (ltype_incl'_use with "Hincl Hl") as "Hl"; first done.
+
+    iPoseProof (ltype_own_has_layout' with "Hl") as "%". { simp_ltype. rewrite Heq_lt. done. }
+    iDestruct ("HT" with "[//] [//]") as "(%Hly' & %Hsz & HT)".
+    
+    iExists _, _. iFrame.
+    assert (syn_type_size_eq (ltype_st lt) st) as ?.
+    { rewrite Hst ltype_st_ofty. 
+      intros ly3 ly4 Hst3 Hst4. 
+      assert (ly3 = ly1) as -> by by eapply syn_type_has_layout_inj.
+      assert (ly4 = ly2) as -> by by eapply syn_type_has_layout_inj.
+      done. }
+    iSplitL.
+    { iMod (ofty_own_split_value_untyped with "Hl") as "(%v & Hv & Hl)"; [done.. | ].
+      iPoseProof (ty_own_ghost_drop with "Hv") as "Hb"; first done.
+      iApply (logical_step_wand with "Hb"). iModIntro. iIntros "$".
+      iApply (ofty_owned_subtype_aligned with "[] Hl"); [done | | ].
+      { done. }
+      iApply owned_type_incl_uninit'; last done.
+      simpl. 
+      intros ?? (-> & _)%syn_type_has_layout_untyped_inv Hst4. 
+      assert (ly2 = ly3) as <- by by eapply syn_type_has_layout_inj. done.
+    }
+    iPureIntro. done.
+  Qed.
+  Global Instance owned_subltype_step_ofty_uninit_inst π E L l {rt} (lt : ltype rt) r st :
+    OwnedSubltypeStep π E L l #r #() lt (◁ uninit st)%I | 101:=
+    λ T, i2p (owned_subltype_step_ofty_uninit π E L lt r st l T).
+
+  (*
+  Lemma owned_subltype_step_ofty_uninit π E L {rt} (lt : ltype rt) r st T :
+    cast_ltype_to_type E L lt (λ ty,
+    li_tactic (compute_layout_goal (ty_syn_type ty)) (λ ly1,
+      li_tactic (compute_layout_goal st) (λ ly2,
+        ⌜ly1 = ly2⌝ ∗ T L (ty_ghost_drop ty π r))))
+    ⊢ owned_subltype_step π E L #r #() lt (◁ uninit st) T.
+  Proof.
+    iDestruct 1 as "(%ty & %Heqt & HT)".
+    rewrite /compute_layout_goal.
+    iDestruct "HT" as "(%ly1 & %Hst1 & %ly2 & %Hst2 & <- & HT)".
+    iIntros (???) "CTX HE HL Hl". simp_ltypes; simpl.
+    iPoseProof (full_eqltype_acc with "CTX HE HL") as "#Hincl"; first apply Heqt.
+    iSpecialize ("Hincl" $! (Owned false) (#r)).
+    iDestruct "Hincl" as "(Hincl & _)". iDestruct "Hincl" as "(%Hst & Hincl & _)".
+    iMod (ltype_incl'_use with "Hincl Hl") as "Hl"; first done.
+    iExists _, _. iFrame.
+    rewrite ltype_own_ofty_unfold /lty_of_ty_own.
+    iDestruct "Hl" as "(%ly & %Halg & %Hly & Hsc & Hlb & _ & %r' & <- & Hb)".
+    assert (ly1 = ly) as -> by by eapply (syn_type_has_layout_inj (ty_syn_type ty)).
+    iMod (fupd_mask_mono with "Hb") as "(%v & Hl & Hv)"; first done.
+    iModIntro. iSplitL.
+    { iPoseProof (ty_own_val_has_layout with "Hv") as "%Hlyv"; first done.
+      iPoseProof (ty_own_ghost_drop with "Hv") as "Hb"; first done.
+      iApply (logical_step_wand with "Hb"). iIntros "$".
+      rewrite ltype_own_ofty_unfold /lty_of_ty_own.
+      iExists _. iR. iR. simpl. iR. iFrame. iR.
+      iExists _. iR. iModIntro. iExists _. iFrame.
+      rewrite uninit_own_spec. eauto. }
+    iPureIntro.
+    iIntros (ly1' ly2' Hst1' Hst2').
+    rewrite Hst in Hst1'. simp_ltypes in Hst1'.
+    assert (ly1' = ly) as -> by by eapply syn_type_has_layout_inj.
+    assert (ly2' = ly) as -> by by eapply syn_type_has_layout_inj.
+    done.
+  Qed.
+  Global Instance owned_subltype_step_ofty_uninit_inst π E L {rt} (lt : ltype rt) r st :
+    OwnedSubltypeStep π E L #r #() lt (◁ uninit st)%I | 101:=
+    λ T, i2p (owned_subltype_step_ofty_uninit π E L lt r st T).
+  *)
+
+  (* TODO move *)
+  Lemma syn_type_has_layout_untyped_mono ly1 ly2 : 
+    ly_align_log ly2 ≤ ly_align_log ly1 →
+    ly_size ly1 = ly_size ly2 →
+    syn_type_has_layout (UntypedSynType ly1) ly1 →
+    syn_type_has_layout (UntypedSynType ly2) ly2.
+  Proof.
+    intros ?? Hut. apply syn_type_has_layout_untyped_inv in Hut as (_ & Hwf & Hsz & Hal).
+    apply syn_type_has_layout_untyped; first done. 
+    - eapply layout_wf_mono; done.
+    - lia.
+    - by eapply ly_align_in_bounds_mono.
+  Qed.
+
+  (* Higher-priority instacne for the special case that we go to Untyped *)
+  Lemma owned_subltype_step_ofty_uninit_untyped π E L l {rt} (lt : ltype rt) r ly T :
+    cast_ltype_to_type E L lt (λ ty,
+      li_tactic (compute_layout_goal (ty_syn_type ty)) (λ ly1,
+      ⌜syn_type_has_layout (ty_syn_type ty) ly1⌝ -∗ 
+      ⌜l `has_layout_loc` ly⌝ ∗
+      ⌜syn_type_has_layout (UntypedSynType ly) ly⌝ ∗
+      (⌜l `has_layout_loc` ly1⌝ -∗
+      ⌜ly_size ly1 = ly_size ly⌝ ∗ T L (ty_ghost_drop ty π r))))
+    ⊢ owned_subltype_step π E L l #r #() lt (◁ uninit (UntypedSynType ly)) T.
+  Proof.
+    iDestruct 1 as "(%ty & %Heqt & HT)".
+    rewrite /compute_layout_goal.
+    iDestruct "HT" as "(%ly1 & %Hst & HT)".
+    iApply owned_subltype_step_ofty_uninit.
+    iExists ty. iR.
+    iExists ly1. iR. iIntros (_). iExists ly.
+    iPoseProof ("HT" with "[//]") as "(%Hly & %Hwf & HT)". 
+    iR. 
+    (*iSplitR. { iPureIntro. *)
+      (*eapply (syn_type_has_layout_untyped_mono ly1); [done.. | ].*)
+      (*by eapply syn_type_has_layout_make_untyped. }*)
+    iIntros (? ?). 
+    iPoseProof ("HT" with "[//]") as "(%Hsz & ?)".
+    iR. iR. done.
+  Qed.
+  Global Instance owned_subltype_step_ofty_uninit_untyped_inst π E L l {rt} (lt : ltype rt) r ly :
+    OwnedSubltypeStep π E L l #r #() lt (◁ uninit (UntypedSynType ly))%I | 100 :=
+    λ T, i2p (owned_subltype_step_ofty_uninit_untyped π E L l lt r ly T).
+  
+  (*
+  Lemma owned_subltype_step_ofty_uninit_untyped π E L {rt} (lt : ltype rt) r ly T :
+    cast_ltype_to_type E L lt (λ ty,
+    ⌜syn_type_has_layout (ty_syn_type ty) ly⌝ ∗ T L (ty_ghost_drop ty π r))
+    ⊢ owned_subltype_step π E L #r #() lt (◁ uninit (UntypedSynType ly)) T.
+  Proof.
+    iDestruct 1 as "(%ty & %Heqt & HT)".
+    iDestruct "HT" as "(%Hst & HT)".
+    iApply owned_subltype_step_ofty_uninit.
+    iExists ty. iR.
+    iExists ly. iR. iExists ly.
+    iSplitR. { iPureIntro. by eapply syn_type_has_layout_make_untyped. }
+    iR. done.
+  Qed.
+  Global Instance owned_subltype_step_ofty_uninit_untyped_inst π E L {rt} (lt : ltype rt) r ly :
+    OwnedSubltypeStep π E L #r #() lt (◁ uninit (UntypedSynType ly))%I | 100 :=
+    λ T, i2p (owned_subltype_step_ofty_uninit_untyped π E L lt r ly T).
+   *)
+
+  (* More specific instances *)
+  Lemma owned_subltype_step_shrltype_uninit π E L {rt} (lt : ltype rt) r st κ l T  :
+    ⌜syn_type_compat PtrSynType st⌝ ∗ T L True%I
+    ⊢ owned_subltype_step π E L l r #() (ShrLtype lt κ) (◁ uninit st) T.
+  Proof.
+    iIntros "(%Hstcomp & HT)".
+    iIntros (??) "CTX HE HL Hl". simp_ltypes; simpl.
+    iMod (ltype_deinit_shr with "Hl") as "Hl"; [done.. | ].
+    iExists _, _. iFrame.
+    iSplitL. { iApply logical_step_intro. by iFrame. }
+    iModIntro. iPureIntro. intros ?? Hst1 Hst2.
+    destruct Hstcomp as [<- | (ly1' & Hst' & ->)]. 
+    + f_equiv. by eapply syn_type_has_layout_inj.
+    + eapply syn_type_has_layout_untyped_inv in Hst2 as (<- & _).
+      f_equiv. by eapply syn_type_has_layout_inj.
+  Qed.
+  Global Instance owned_subltype_step_shrltype_uninit_inst π E L {rt} (lt : ltype rt) r st κ l :
+    OwnedSubltypeStep π E L l (r) #() (ShrLtype lt κ) (◁ uninit st)%I | 20 :=
+    λ T, i2p (owned_subltype_step_shrltype_uninit π E L lt r st κ l T).
+
+  Lemma owned_subltype_step_mutltype_uninit π E L {rt} (lt : ltype rt) r γ st κ l T  :
+    match ltype_uniq_extractable lt with
+    | None => False
+    | Some κm =>
+        ⌜syn_type_compat PtrSynType st⌝ ∗ T L (MaybeInherit κm InheritGhost (place_rfn_interp_mut_extracted r γ))
+    end
+    ⊢ owned_subltype_step π E L l #(r, γ) #() (MutLtype lt κ) (◁ uninit st) T.
+  Proof.
+    iIntros "HT".
+    iIntros (??) "CTX HE HL Hl". simp_ltypes; simpl.
+    destruct (ltype_uniq_extractable lt) eqn:Hextract; last done.
+    iDestruct "HT" as "(%Hstcomp & HT)".
+    iExists _, _. iFrame.
+    iMod (ltype_uniq_extractable_deinit_mut with "Hl") as "(Hl & Hf)"; [done.. | ].
+    iPoseProof (MaybeInherit_update (place_rfn_interp_mut_extracted r γ) with "[] Hf") as "Hf".
+    { iIntros (?) "Hrfn". iMod (place_rfn_interp_mut_extract with "Hrfn") as "?". done. }
+    iModIntro. iSplitL. { iApply logical_step_intro. iFrame. }
+    iPureIntro. iIntros (ly1 ly2 Halg1 Halg2).
+    specialize (syn_type_compat_layout_trans _ _ _ Hstcomp Halg2) as ?.
+    f_equiv. by eapply syn_type_has_layout_inj.
+  Qed.
+  Global Instance owned_subltype_step_mutltype_uninit_inst π E L {rt} (lt : ltype rt) r γ st κ l :
+    OwnedSubltypeStep π E L l #(r, γ) #() (MutLtype lt κ) (◁ uninit st)%I | 20 :=
+    λ T, i2p (owned_subltype_step_mutltype_uninit π E L lt r γ st κ l T).
+
+  (*Lemma owned_subltype_step_cast_to_type_uninit : *)
+    (*cast_ltype_to_type E L lt (λ ty, *)
+      (*⌜syn_type_compat (ty_syn_type ty) st⌝ ∗ T L (ty_ghost_drop ty)) -∗*)
+    (*owned_subltype_step π E L r #() lt (◁ uninit st) T.*)
+
+  (* TODO have fallback instance that uses cast_ltype *)
+
+  (* TODO more instances for other ltypes under which borrows can happen, e.g. for structs *)
+
+  (* Fallback without a logical step -- here, we cannot ghost_drop *)
+  (* TODO: maybe restrict this instance more for earlier failure *)
+  Lemma uninit_mono E L l {rt} (ty : type rt) r π st T :
+    (li_tactic (compute_layout_goal st) (λ ly, ⌜syn_type_has_layout ty.(ty_syn_type) ly⌝ ∗ (∀ v, v ◁ᵥ{π} r @ ty -∗ T L True%I)))
+    ⊢ subsume_full E L false (l ◁ₗ[π, Owned false] #r @ (◁ ty)) (l ◁ₗ[π, Owned false] .@ (◁ (uninit st))) T.
+  Proof.
+    rewrite /compute_layout_goal.
+    iIntros "(%ly & %Halg1 & %Halg2 & HT)".
+    iIntros (???) "#CTX #HE HL Hl".
+    rewrite !ltype_own_ofty_unfold /lty_of_ty_own. simpl.
+    iDestruct "Hl" as "(%ly' & %Halg & %Hly & Hsc & ? & ? & %r' & <- & Hv)".
+    iMod (fupd_mask_mono with "Hv") as "(%v & Hl & Hv)"; first done.
+    iPoseProof (ty_own_val_has_layout with "Hv") as "%"; first done.
+    iExists L, True%I. iPoseProof ("HT" with "Hv") as "$". iFrame "HL".
+    rewrite right_id. assert (ly' = ly) as -> by by eapply syn_type_has_layout_inj.
+    rewrite ltype_own_ofty_unfold /lty_of_ty_own. simpl.
+    iExists ly. iSplitR; first done. iSplitR; first done.
+    iSplitR; first done. iFrame. iExists _. iSplitR; first done.
+    iModIntro. iModIntro. iExists v. iFrame.
+    iExists ly. iSplitR; first done. iSplitR; first done.
+    iPureIntro. rewrite Forall_forall. done.
+  Qed.
+  Global Instance uninit_mono_inst π E L l {rt} (ty : type rt) (r : rt) st :
+    SubsumeFull E L false (l ◁ₗ[π, Owned false] PlaceIn r @ (◁ ty))%I (l ◁ₗ[π, Owned false] .@ ◁ (uninit st))%I | 40 :=
+    λ T, i2p (uninit_mono E L l ty r π st T).
+
 
   (** We have this instance because it even works when [r1 = PlaceGhost ..] *)
   Lemma weak_subltype_deinit E L {rt1} (r1 : place_rfn rt1) r2 (ty : type rt1) st T :
